theories/LogicalRelation/ShapeView.v
@@ -13,9 +13,9 @@ Section ShapeViews.
 (** A shape view is inhabited exactly on the diagonal, ie when the two types are reducible
   in the same way. *)
 
-  Definition ShapeView@{i j k l i' j' k' l'} Γ
+  Definition ShapeView@{i j k l i' j' k' l'} Γ sA sB
     A {lA eqTyA redTmA redTyA} B {lB eqTyB redTmB redTyB}
-    (lrA : LogRel@{i j k l} lA Γ A eqTyA redTmA redTyA) (lrB : LogRel@{i' j' k' l'} lB Γ B eqTyB redTmB redTyB) : Set :=
+    (lrA : LogRel@{i j k l} lA Γ sA A eqTyA redTmA redTyA) (lrB : LogRel@{i' j' k' l'} lB Γ sB B eqTyB redTmB redTyB) : Set :=
     match lrA, lrB with
       | LRU _ _, LRU _ _ => True
       | LRne _ _, LRne _ _ => True
@@ -27,7 +27,7 @@ Section ShapeViews.
       | _, _ => False
     end.
 
-  Arguments ShapeView Γ A {lA eqTyA redTmA redTyA} B {lB eqTyB redTmB redTyB}
+  Arguments ShapeView Γ sA sB A {lA eqTyA redTmA redTyA} B {lB eqTyB redTmB redTyB}
   !lrA !lrB.
 
 (** ** The main property *)
@@ -37,34 +37,37 @@ if two reducible types are reducibly convertible, then they must be reducible in
 This lets us relate different reducibility proofs when we have multiple such proofs, typically
 when showing symmetry or transitivity of the logical relation. *)
 
-  Arguments ShapeView Γ A {lA eqTyA redTmA redTyA} B {lB eqTyB redTmB redTyB}
+  Arguments ShapeView Γ sA sB A {lA eqTyA redTmA redTyA} B {lB eqTyB redTmB redTyB}
   !lrA !lrB.
 
 
-  Lemma red_whnf@{i j k l} {Γ A lA eqTyA redTmA eqTmA}
-    (lrA : LogRel@{i j k l} lA Γ A eqTyA redTmA eqTmA) : 
-    ∑ nf, [Γ |- A :⤳*: nf] × whnf nf.
+  Lemma red_whnf@{i j k l} {Γ s A lA eqTyA redTmA eqTmA}
+    (lrA : LogRel@{i j k l} lA Γ s A eqTyA redTmA eqTmA) : 
+    ∑ nf, [Γ |- A :⤳*: nf @ s] × whnf nf.
   Proof.
-    pattern lA, Γ, A, eqTyA, redTmA, eqTmA, lrA; eapply LR_rect; intros ??[].
-    all: eexists; split; tea; constructor; tea.
+    pattern lA, Γ, s, A, eqTyA, redTmA, eqTmA, lrA; eapply LR_rect.
+    2: intros ?.
+    all: intros ??[]; eexists; split; tea; constructor; tea.
     now eapply convneu_whne.
   Defined.
 
-  Lemma eqTy_red_whnf@{i j k l} {Γ A lA eqTyA redTmA eqTmA B}
-    (lrA : LogRel@{i j k l} lA Γ A eqTyA redTmA eqTmA) : 
-    eqTyA B -> ∑ nf, [Γ |- B :⤳*: nf] × whnf nf.
+  Lemma eqTy_red_whnf@{i j k l} {Γ s A lA eqTyA redTmA eqTmA B}
+    (lrA : LogRel@{i j k l} lA Γ s A eqTyA redTmA eqTmA) : 
+    eqTyA B -> ∑ nf, [Γ |- B :⤳*: nf @ s] × whnf nf.
   Proof.
-    pattern lA, Γ, A, eqTyA, redTmA, eqTmA, lrA.
-    eapply LR_rect_LogRelRec@{i j k l k}; intros ??? [].
+    pattern lA, Γ, s, A, eqTyA, redTmA, eqTmA, lrA.
+    eapply LR_rect_LogRelRec@{i j k l k}.
+    2: intros ?.
+    all: intros ??? [].
     3,6,7: intros ??.
     all: intros []; eexists; split; tea; constructor; tea.
     eapply convneu_whne; now symmetry.
   Defined.
 
-  Lemma ShapeViewConv@{i j k l i' j' k' l'} {Γ A lA eqTyA redTmA eqTmA B lB eqTyB redTmB eqTmB}
-    (lrA : LogRel@{i j k l} lA Γ A eqTyA redTmA eqTmA) (lrB : LogRel@{i' j' k' l'} lB Γ B eqTyB redTmB eqTmB) :
+  Lemma ShapeViewConv@{i j k l i' j' k' l'} {Γ sA sB A lA eqTyA redTmA eqTmA B lB eqTyB redTmB eqTmB}
+    (lrA : LogRel@{i j k l} lA Γ sA A eqTyA redTmA eqTmA) (lrB : LogRel@{i' j' k' l'} lB Γ sB B eqTyB redTmB eqTmB) :
     eqTyA B ->
-    ShapeView@{i j k l i' j' k' l'} Γ A B lrA lrB.
+    ShapeView@{i j k l i' j' k' l'} Γ sA sB A B lrA lrB.
   Proof.
     intros eqAB.
     pose (x := eqTy_red_whnf lrA eqAB).
@@ -72,7 +75,7 @@ when showing symmetry or transitivity of the logical relation. *)
     pose proof (h := redtywf_det (snd x.π2) (snd y.π2) (fst x.π2) (fst y.π2)).
     revert eqAB x y h. 
     destruct lrA; destruct lrB; intros []; cbn; try easy; try discriminate.
-    all: try now (intros e; destruct neA as [? ? ne]; subst; apply convneu_whne in ne; inversion ne).
+    all: try now (intros e; destruct neA as [? ? ? ne]; subst; apply convneu_whne in ne; inversion ne).
     all: try now (intros e; subst; symmetry in eq; apply convneu_whne in eq; inversion eq).
   Qed.
 
